experiment with a version of inhale_rel that can reason about optimizations that use knowledge on assertions
generalized the general composition and conditional rules to achieve simple proofs for rules deriving the new inhale_rel definition

InhaleRel.thy
@@ -15,7 +15,7 @@ definition inhale_rel ::
            (\<lambda> \<omega> \<omega>'. red_inhale ctxt_vpr StateCons assertion_vpr \<omega> (RNormal \<omega>'))
            (\<lambda> \<omega>. red_inhale ctxt_vpr StateCons assertion_vpr \<omega> RFailure)
            P ctxt \<gamma> \<gamma>'"
-
+    
 lemma inhale_rel_intro:
   assumes
     "\<And>\<omega> ns \<omega>'. 
@@ -61,6 +61,76 @@ lemma inhale_rel_failure_elim:
   unfolding inhale_rel_def rel_general_def
   by auto
 
+subsection \<open>Inhale rel definition that can handle optimizations\<close>
+
+definition inhale_opt_rel ::
+     "('a full_total_state \<Rightarrow> 'a vbpl_absval nstate \<Rightarrow> bool)
+     \<Rightarrow> ((pure_exp, pure_exp atomic_assert) assert \<Rightarrow> 'a full_total_state \<Rightarrow> bool)
+     \<Rightarrow> 'a total_context
+        \<Rightarrow> ('a full_total_state \<Rightarrow> bool)
+           \<Rightarrow> bigblock list
+                    \<Rightarrow> 'a econtext_bpl
+                       \<Rightarrow> (pure_exp, pure_exp atomic_assert) assert
+                          \<Rightarrow> bigblock \<times> cont \<Rightarrow> bigblock \<times> cont \<Rightarrow> bool"
+  where "inhale_opt_rel R Q ctxt_vpr StateCons P ctxt assertion_vpr \<gamma> \<gamma>' \<equiv>
+         rel_general (\<lambda> \<omega> ns. R \<omega> ns \<and> Q assertion_vpr \<omega>)  R 
+           (\<lambda> \<omega> \<omega>'. red_inhale ctxt_vpr StateCons assertion_vpr \<omega> (RNormal \<omega>'))
+           (\<lambda> \<omega>. red_inhale ctxt_vpr StateCons assertion_vpr \<omega> RFailure)
+           P ctxt \<gamma> \<gamma>'"
+
+definition is_assertion_red_invariant
+  where "is_assertion_red_invariant ctxt StateCons Q Success \<equiv>
+          (\<forall> A1 A2 \<omega>. Q (A1 && A2) \<omega> \<longrightarrow> 
+                  (Q A1 \<omega>) \<and>
+                  (\<forall>\<omega>'. Success A1 \<omega> \<omega>' \<longrightarrow> Q A2 \<omega>')) \<and>
+          (\<forall> e A \<omega>. Q (assert.Imp e A) \<omega> \<longrightarrow> ctxt, StateCons, Some \<omega> \<turnstile> \<langle>e; \<omega>\<rangle> [\<Down>]\<^sub>t (Val (VBool True)) \<longrightarrow> Q A \<omega>)"
+
+lemma is_assertion_red_invariant_intro:
+  assumes "\<And> A1 A2 \<omega>. Q (A1 && A2) \<omega> \<Longrightarrow> Q A1 \<omega>" and
+          "\<And> A1 A2 \<omega> \<omega>'. Q (A1 && A2) \<omega> \<Longrightarrow> Success A1 \<omega> \<omega>' \<Longrightarrow> Q A2 \<omega>'" and
+          "\<And> e A \<omega>. Q (assert.Imp e A) \<omega> \<Longrightarrow> 
+                    ctxt, StateCons, Some \<omega> \<turnstile> \<langle>e; \<omega>\<rangle> [\<Down>]\<^sub>t (Val (VBool True)) \<Longrightarrow> Q A \<omega>"
+        shows "is_assertion_red_invariant ctxt StateCons Q Success"
+  using assms
+  unfolding is_assertion_red_invariant_def
+  by blast
+
+definition is_assertion_red_invariant_inh
+  where "is_assertion_red_invariant_inh ctxt_vpr StateCons Q \<equiv> 
+              is_assertion_red_invariant ctxt_vpr StateCons Q (\<lambda>A \<omega> \<omega>'. red_inhale ctxt_vpr StateCons A \<omega> (RNormal \<omega>'))"
+
+lemma is_assertion_red_invariant_inh:
+  "is_assertion_red_invariant_inh ctxt_vpr StateCons (assertion_framing_state ctxt_vpr StateCons)"
+  unfolding is_assertion_red_invariant_inh_def 
+  apply (rule is_assertion_red_invariant_intro)
+  by (blast dest: assertion_framing_star assertion_framing_imp)+
+
+lemma expr_wf_rel_inh_opt:
+  assumes "\<And> \<omega>def \<omega> ns. R \<omega>def \<omega> ns \<Longrightarrow> \<omega>def = \<omega> \<and> assertion_framing_state ctxt_vpr StateCons (Atomic A) \<omega>def" and
+          "es = sub_expressions_atomic A" and
+          "es \<noteq> []"
+        shows  "exprs_wf_rel R ctxt_vpr StateCons P ctxt es \<gamma> \<gamma>"
+  unfolding exprs_wf_rel_def
+proof (rule wf_rel_intro)
+  fix contra
+  fix \<omega>def \<omega> ns
+  assume "R \<omega>def \<omega> ns" and RedExps: "red_pure_exps_total ctxt_vpr StateCons (Some \<omega>def) es \<omega> None"
+  hence "red_inhale ctxt_vpr StateCons (Atomic A) \<omega>def RFailure"
+    using assms InhSubAtomicFailure
+    by blast
+
+  moreover from \<open>R \<omega>def \<omega> ns\<close> have "assertion_framing_state ctxt_vpr StateCons (Atomic A) \<omega>def"
+    using assms
+    by blast
+
+  ultimately have False
+    unfolding assertion_framing_state_def
+    by blast
+
+  thus contra
+    by blast
+qed (blast intro: red_ast_bpl_refl)
+
 subsection \<open>Propagation rules\<close>
 
 lemma inhale_propagate_pre:
@@ -90,6 +160,41 @@ lemma inhale_rel_star:
   apply (rule rel_general_comp)
   by (auto elim: InhStar_case)
 
+lemma inhale_opt_rel_star:
+  assumes Invariant1: "\<And> \<omega>. Q (A1 && A2) \<omega> \<Longrightarrow> Q A1 \<omega>" and
+          Invariant2: "\<And> \<omega> \<omega>'. Q (A1 && A2) \<omega> \<Longrightarrow> red_inhale ctxt_vpr StateCons A1 \<omega> (RNormal \<omega>') \<Longrightarrow> Q A2 \<omega>'" and
+          RelA1: "inhale_opt_rel R Q ctxt_vpr StateCons P ctxt A1 \<gamma>1 \<gamma>2" and
+          RelA2: "inhale_opt_rel R Q ctxt_vpr StateCons P ctxt A2 \<gamma>2 \<gamma>3"
+  shows "inhale_opt_rel R Q ctxt_vpr StateCons P ctxt (A1 && A2) \<gamma>1 \<gamma>3"
+  text\<open>Idea of proof:
+       \<^item> use general composition rule where the intermediate relation is chosen to be \<^term>\<open>\<lambda>\<omega> ns. R \<omega> ns \<and> Q A2 \<omega>\<close>
+       \<^item> Prove the first premise by weakening the input relation from \<^term>\<open>\<lambda>\<omega> ns. R \<omega> ns \<and> Q (A1 && A2) \<omega>\<close> to \<^term>\<open>\<lambda>\<omega> ns. R \<omega> ns \<and> Q A1 \<omega>\<close>
+         and by adjusting the output relation \<^term>\<open>\<lambda>\<omega> ns. R \<omega> ns \<and> Q A2 \<omega>\<close> to \<^term>\<open>R\<close> (\<^term>\<open>R\<close> is strong enough
+         to recover \<^term>\<open>\<lambda>\<omega> ns. R \<omega> ns \<and> Q A2 \<omega>\<close>)\<close>
+  unfolding inhale_opt_rel_def
+  apply (rule rel_general_comp[where ?R2.0="\<lambda>\<omega> ns. R \<omega> ns \<and> Q A2 \<omega>"])
+     apply (rule rel_general_conseq_input_output)
+       apply (rule RelA1[simplified inhale_opt_rel_def])
+      apply (simp add: Invariant1)
+     apply (fastforce dest: Invariant2)
+    apply (rule RelA2[simplified inhale_opt_rel_def])
+  by (auto elim: InhStar_case)
+
+lemma inhale_opt_rel_star_2:
+  assumes Invariant: "is_assertion_red_invariant_inh ctxt_vpr StateCons Q" and
+          RelA1: "inhale_opt_rel R Q ctxt_vpr StateCons P ctxt A1 \<gamma>1 \<gamma>2" and
+          RelA2: "inhale_opt_rel R Q ctxt_vpr StateCons P ctxt A2 \<gamma>2 \<gamma>3"
+        shows "inhale_opt_rel R Q ctxt_vpr StateCons P ctxt (A1 && A2) \<gamma>1 \<gamma>3"
+  apply (rule inhale_opt_rel_star)
+  using Invariant 
+  unfolding is_assertion_red_invariant_inh_def is_assertion_red_invariant_def
+     apply blast
+  using Invariant 
+  unfolding is_assertion_red_invariant_inh_def is_assertion_red_invariant_def
+    apply blast
+  using assms
+  by auto
+
 lemma inhale_rel_imp:
   assumes 
    ExpWfRel:          
@@ -114,8 +219,8 @@ next
   fix \<omega> \<omega>' ns
   assume "red_inhale ctxt_vpr StateCons (assert.Imp cond A) \<omega> (RNormal \<omega>')" and "R \<omega> ns"
   thus "((\<exists>v. ctxt_vpr, StateCons, Some \<omega> \<turnstile> \<langle>cond;\<omega>\<rangle> [\<Down>]\<^sub>t Val v) \<and> \<omega> = \<omega>) \<and>
-       (red_expr_bpl ctxt cond_bpl ns (BoolV True) \<and> red_inhale ctxt_vpr StateCons A \<omega> (RNormal \<omega>') \<or>
-        red_expr_bpl ctxt cond_bpl ns (BoolV False) \<and> \<omega> = \<omega>')"
+       (red_expr_bpl ctxt cond_bpl ns (BoolV True) \<and> R \<omega> ns \<and> red_inhale ctxt_vpr StateCons A \<omega> (RNormal \<omega>') \<or>
+        red_expr_bpl ctxt cond_bpl ns (BoolV False) \<and> R \<omega> ns \<and> \<omega> = \<omega>')"
     apply (cases)
     using exp_rel_vpr_bpl_elim_2[OF ExpRel]
     apply (metis val_rel_vpr_bpl.simps(2))
@@ -126,12 +231,55 @@ next
   assume "red_inhale ctxt_vpr StateCons (assert.Imp cond A) \<omega> RFailure" and "R \<omega> ns"
   thus "ctxt_vpr, StateCons, Some \<omega> \<turnstile> \<langle>cond;\<omega>\<rangle> [\<Down>]\<^sub>t VFailure \<or>
        ((\<exists>v. ctxt_vpr, StateCons, Some \<omega> \<turnstile> \<langle>cond;\<omega>\<rangle> [\<Down>]\<^sub>t Val v) \<and> \<omega> = \<omega>) \<and>
-       (red_expr_bpl ctxt cond_bpl ns (BoolV True) \<and> red_inhale ctxt_vpr StateCons A \<omega> RFailure \<or>
-        red_expr_bpl ctxt cond_bpl ns (BoolV False) \<and> False)"
+       (red_expr_bpl ctxt cond_bpl ns (BoolV True) \<and> R \<omega> ns \<and> red_inhale ctxt_vpr StateCons A \<omega> RFailure \<or>
+        red_expr_bpl ctxt cond_bpl ns (BoolV False) \<and> R \<omega> ns \<and> False)"
     apply (cases)
     using exp_rel_vpr_bpl_elim_2[OF ExpRel]
      apply (metis val_rel_vpr_bpl.simps(2))
     by auto
+qed
+
+lemma inhale_opt_rel_imp:
+  assumes 
+   Invariant: "\<And>\<omega>. ctxt_vpr, StateCons, Some \<omega> \<turnstile> \<langle>cond; \<omega>\<rangle> [\<Down>]\<^sub>t (Val (VBool True)) \<Longrightarrow> Q (assert.Imp cond A) \<omega> \<Longrightarrow> Q A \<omega>" and
+   ExpWfRel:          
+        "expr_wf_rel (\<lambda> \<omega>def \<omega> ns. \<omega>def = \<omega> \<and> R \<omega> ns \<and> Q (assert.Imp cond A) \<omega>) ctxt_vpr StateCons P ctxt cond 
+         \<gamma>1
+         (if_bigblock name (Some (cond_bpl)) (thn_hd # thn_tl) [empty_else_block], KSeq next cont)" 
+        (is "expr_wf_rel _ ctxt_vpr StateCons P ctxt cond _ ?\<gamma>_if") and
+   EmptyElse: "is_empty_bigblock empty_else_block" and
+   ExpRel: "exp_rel_vpr_bpl (\<lambda> \<omega>def \<omega> ns. \<omega>def = \<omega> \<and> R \<omega> ns) ctxt_vpr ctxt cond cond_bpl" and
+   RhsRel: "inhale_opt_rel R Q ctxt_vpr StateCons P ctxt A (thn_hd, convert_list_to_cont thn_tl (KSeq next cont)) (next, cont)"
+                (is "inhale_opt_rel R Q _ _ _ _ _ ?\<gamma>_thn (next, cont)")
+              shows "inhale_opt_rel R Q ctxt_vpr StateCons P ctxt (assert.Imp cond A) \<gamma>1 (next, cont)"
+  unfolding inhale_opt_rel_def
+proof (rule rel_general_cond,
+       fastforce intro: rel_general_conseq_input_output[OF wf_rel_general_1[OF ExpWfRel]],
+       rule RhsRel[simplified inhale_opt_rel_def])
+  show "rel_general R R (\<lambda> \<omega> \<omega>'. \<omega> = \<omega>') (\<lambda>_. False) P ctxt (empty_else_block, convert_list_to_cont [] (KSeq next cont)) (next, cont)"
+    apply (rule rel_intro)
+    using red_ast_bpl_empty_block_2[OF EmptyElse]
+    apply fastforce
+    by simp
+next
+  fix \<omega> \<omega>' ns
+  assume "red_inhale ctxt_vpr StateCons (assert.Imp cond A) \<omega> (RNormal \<omega>')" and "R \<omega> ns \<and> Q (assert.Imp cond A) \<omega>"
+  thus "((\<exists>v. ctxt_vpr, StateCons, Some \<omega> \<turnstile> \<langle>cond;\<omega>\<rangle> [\<Down>]\<^sub>t Val v) \<and> \<omega> = \<omega>) \<and>
+       (red_expr_bpl ctxt cond_bpl ns (BoolV True) \<and> (R \<omega> ns \<and> Q A \<omega>) \<and> red_inhale ctxt_vpr StateCons A \<omega> (RNormal \<omega>') \<or>
+        red_expr_bpl ctxt cond_bpl ns (BoolV False) \<and> R \<omega> ns \<and> \<omega> = \<omega>')"
+    apply (cases)
+    using ExpRel
+    by (fastforce elim: exp_rel_vpr_bpl_elim_2 simp: Invariant)+
+next
+  fix \<omega> ns
+  assume "red_inhale ctxt_vpr StateCons (assert.Imp cond A) \<omega> RFailure" and "R \<omega> ns \<and> Q (assert.Imp cond A) \<omega>"
+  thus "ctxt_vpr, StateCons, Some \<omega> \<turnstile> \<langle>cond;\<omega>\<rangle> [\<Down>]\<^sub>t VFailure \<or>
+       ((\<exists>v. ctxt_vpr, StateCons, Some \<omega> \<turnstile> \<langle>cond;\<omega>\<rangle> [\<Down>]\<^sub>t Val v) \<and> \<omega> = \<omega>) \<and>
+       (red_expr_bpl ctxt cond_bpl ns (BoolV True) \<and> (R \<omega> ns \<and> Q A \<omega>) \<and> red_inhale ctxt_vpr StateCons A \<omega> RFailure \<or>
+        red_expr_bpl ctxt cond_bpl ns (BoolV False) \<and> R \<omega> ns \<and> False)"
+    apply (cases)
+    using ExpRel
+    by (fastforce elim: exp_rel_vpr_bpl_elim_2 simp: Invariant)+
 qed
 
 subsection \<open>Field access predicate rule\<close>
@@ -143,7 +291,7 @@ definition inhale_acc_normal_premise
        p \<ge> 0 \<and>
        (p > 0 \<longrightarrow> r \<noteq> Null) \<and>
        (let W' = (if r = Null then {\<omega>} else inhale_perm_single StateCons \<omega> (the_address r,f) (Some (Abs_prat p))) in
-       (W' \<noteq> {} \<and> \<omega>' \<in> W'))"                       
+       (W' \<noteq> {} \<and> \<omega>' \<in> W'))" 
 
 lemma inhale_field_acc_rel:
   assumes 
