TotalExpressions.thy
@@ -696,5 +696,12 @@ next
   qed
 qed
 
+lemma assertion_framing_imp: 
+  assumes "assertion_framing_state ctxt StateCons (Imp e A) \<omega>" and
+          "ctxt, StateCons, Some \<omega> \<turnstile> \<langle>e; \<omega>\<rangle> [\<Down>]\<^sub>t (Val (VBool True))"  
+        shows "assertion_framing_state ctxt StateCons A \<omega>"
+  using assms
+  unfolding assertion_framing_state_def
+  by (auto intro: InhImpTrue)
 
 end
